Source/DafnyCore/AST/TypeDeclarations/TopLevelDeclWithMembers.cs
@@ -249,7 +249,7 @@ public abstract class TopLevelDeclWithMembers : TopLevelDecl, IHasSymbolChildren
           extraMember.InheritVisibility(m, false);
           members.Add(extraName.Value, extraMember);
         } else if (m is Function f && f.ByMethodBody != null) {
-          ModuleResolver.RegisterByMethod(f, this);
+          resolver.RegisterByMethod(f, this);
         }
       } else if (m is Constructor && !((Constructor)m).HasName) {
         resolver.reporter.Error(MessageSource.Resolver, m, "More than one anonymous constructor");
