Source/DafnyCore/DafnyOptions.cs
@@ -125,6 +125,10 @@ NoGhost - disable printing of functions, ghost methods, and proof
       }
 
       RegisterLegacyUi(CommonOptionBag.AddCompileSuffix, ParseBoolean, "Compilation options", "compileSuffix");
+      
+      RegisterLegacyUi(CommonOptionBag.ReadsClausesOnMethods, ParseBoolean, "Language feature selection", "readsClausesOnMethods", @"
+0 (default) - Reads clauses on methods are forbidden.
+1 - Reads clauses on methods are permitted.".TrimStart(), defaultValue: false);
     }
 
     public void ApplyBinding(Option option) {
