Test/dafny0/ReadsOnMethods.dfy
@@ -1,4 +1,4 @@
-// RUN: %exits-with 4 %dafny /compile:0 /deprecation:0 "%s" > "%t"
+// RUN: %exits-with 4 %dafny /compile:0 /readsClausesOnMethods:1 "%s" > "%t"
 // RUN: %diff "%s.expect" "%t"
 
 // The first half of this file is a clone of Reads.dfy, 
@@ -8,7 +8,7 @@
 
 // Checking that the reads clause also is checked over requires
 
-class C { var u : int; }
+class C { var u : int }
 
 // Unlike functions, the default for methods is * instead of {}
 ghost method yup1(c : C)
@@ -47,7 +47,7 @@ ghost method nope3(xs : seq<C>)
 
 ghost method ok3(xs : seq<C>)
      requires |xs| > 0 && xs[0].u > 0
-     reads xs;
+     reads xs
 {}
 
 ghost method nope4(c : C, xs : set<C>)
@@ -156,6 +156,8 @@ ghost method FunctionInQuantifier2() returns (r: int)
   reads {}
   ensures r == 100
 {
+  // BUG: f.reads(10) is flagged for some reason. 
+  // The wellformedness checks for LetSuchThat may be subtley different than AssignSuchThat...
   var f: int ~> int :| f.reads(10) == {} && f.requires(10) && f(10) == 100;  // fine :) :)
   return f(10);
 }
@@ -185,3 +187,219 @@ class ReadsTestsInsideLetSuchThat {
 
 // And now for brand new freshly-baked tests!
 
+class Box<T> {
+  var x: T
+
+  constructor(x: T)
+    reads {}
+  {
+    this.x := x;
+  }
+}
+
+method SetBox(b: Box<int>, i: int) 
+  reads b
+  modifies b
+{
+  b.x := i;
+}
+
+function GetBoxFn(b: Box<int>): int
+  reads b
+{
+  b.x
+}
+
+method GetBoxCorrectReads(b: Box<int>) returns (i: int)
+  reads b
+{
+  i := b.x;
+}
+
+method GetBoxReadsStar(b: Box<int>) returns (i: int)
+  reads *
+{
+  i := b.x;
+}
+
+method GetBoxIncorrectReads(b: Box<int>) returns (i: int)
+  reads {}
+{
+  i := b.x; // Error: insufficient reads clause to read field
+}
+
+method GetBoxDefaultReads(b: Box<int>) returns (i: int)
+{
+  i := b.x;
+}
+
+method ReadingAndWritingFreshStateAllowed()
+  reads {}
+{
+  var myBox := new Box(42);
+  var x := GetBoxFn(myBox);
+  SetBox(myBox, 42);
+}
+
+method ApplyLambda<T(!new), R>(f: T ~> R, t: T) returns (r: R) 
+  requires f.requires(t)
+  reads f.reads
+{
+  r := f(t);
+}
+
+// method DependsOnAllocationState<T>(b: Box<T>) 
+//   reads set t: T :: b // BUG? This isn't allowed on functions...
+// {
+// }
+
+datatype Option<T> = Some(value: T) | None
+
+class {:extern} ExternalSequentialMutableMap<K, V> {
+  ghost var state: map<K, V>
+  method {:extern} Put(k: K, v: V)
+    requires k !in state
+    modifies this
+    ensures state == old(state)[k := v]
+  function {:extern} Get(k: K): (v: Option<V>)
+    reads this
+    ensures k in state ==> v == Some(state[k])
+    ensures k !in state ==> v == None
+}
+
+method {:concurrent} MemoizedSquare2(x: int, cache: ExternalSequentialMutableMap<int, int>) returns (xSquared: int)
+  requires forall k | k in cache.state :: cache.state[k] == k * k   // Error: insufficient reads clause to read field
+  reads {}
+  ensures xSquared == x * x
+{
+  var cached := cache.Get(x);  // Error: insufficient reads clause to invoke function
+  if cached.Some? {
+    xSquared := cached.value;
+  } else {
+    xSquared := x * x;
+    cache.Put(x, xSquared);    // Error: call might violate context's modifies clause
+                               // Error: insufficient reads clause to call
+  }
+}
+
+class {:extern} ExternalConcurrentMutableMap<K, V> {
+  const inv: (K, V) -> bool
+  method {:extern} Put(k: K, v: V)
+    reads {}
+    requires inv(k, v)
+  method {:extern} Get(k: K) returns (v: Option<V>)
+    reads {}
+    ensures v.Some? ==> inv(k, v.value)
+}
+
+method {:concurrent} MemoizedSquare(x: int, cache: ExternalConcurrentMutableMap<int, int>) returns (xSquared: int)
+  requires cache.inv == ((key, value) => value == key * key)
+  reads {}
+  ensures xSquared == x * x
+{
+  var cached := cache.Get(x);
+  if cached.Some? {
+    xSquared := cached.value;
+  } else {
+    xSquared := x * x;
+    cache.Put(x, xSquared);
+  }
+}
+
+function Always42(b: Box<int>): int {
+  42
+} by method {
+  var result := 42;
+  result := result + b.x; // Error: insufficient reads clause to read field
+  result := result - b.x;
+  return 42;
+}
+
+method BadMetaBox(b: Box<Box<int>>)
+  reads {}
+  modifies b.x  // Error: insufficient reads clause to read field
+{
+  b.x.x := 42;  // Error: insufficient reads clause to read field
+}
+
+method GoodMetaBox(b: Box<Box<int>>)
+  modifies b.x
+{
+  b.x.x := 42;
+}
+
+function GoodMetaBox2(b: Box<Box<int>>): int
+  reads b, b.x
+{
+  b.x.x
+}
+
+trait MyTrait {
+  method M(b: Box<int>) returns (r: int)
+    reads {}
+}
+
+class MyClass extends MyTrait {
+  method M(b: Box<int>) returns (r: int) // Error: method might read an object not in the parent trait context's reads clause
+    reads b
+  {
+    return 42;
+  }
+}
+
+// Testing the reads checks on other clauses
+method OnlySpecReads(b: Box<int>) returns (r: int)
+  requires b.x == 42  // Error: insufficient reads clause to read field
+  reads {}
+  ensures r == b.x
+{
+  return 42;
+}
+
+method DefaultValueReads(b: Box<int>, x: int := b.x)  // Error: insufficient reads clause to read field
+  returns (r: int)
+  reads {}
+{
+  return 42;
+}
+
+// TODO:
+// * Array reads!
+// * Ensuring LHS' aren't checked as reads (LValueContext) - this.x working, array setting not working
+//   * Lots of cases!
+// * Invoking twostate things from methods
+// * Example for the need to add fresh loop invariants in functions by methods?
+// * Double check refinement
+// * Missing check for reads clause not allowed to depend on set of allocated objects (?)
+// * Double-check if it's correct that function default values don't assume preconditions (see example below)
+// * Document explicit choice not to change autocontracts (?)
+// * Figure out FunctionInQuantifier2 method
+//   * Something to do with difference between AssignSuchThat and LetSuchThat?
+//   * Possibly just leave and ask in PR review
+
+// FUTURE:
+// * Optimize checking for `reads {}`? Can be checked with a simple AST pass, much cheaper
+//   * At least some cases might be handled by existing IsAlwaysTrue
+// * Document explicit choice not to include method reads clause in decreases clause
+
+
+function Partition(s: seq<int>, p: int -> bool, a: array<int>): (seq<int>, seq<int>) {
+  ([], [])
+} by method {
+  var b := new int[10];
+  var loop := true;
+  while loop
+    decreases loop
+  {
+    b[0] := 42;
+    loop := false;
+  }
+  b[0] := 42;
+  return ([], []);
+}
+
+// function DefaultValue(b: int, v: int := 1 / b): int 
+//   requires b != 0
+// {
+//   42
+// }
