Test/dafny0/ConcurrentAttribute.dfy
@@ -1,0 +1,56 @@
+// RUN: %exits-with 4 %verify --reads-clauses-on-methods "%s" > "%t"
+// RUN: %diff "%s.expect" "%t"
+
+class Box<T> {
+  var x: T
+
+  constructor(x: T)
+    reads {}
+  {
+    this.x := x;
+  }
+}
+
+class Concurrent {
+
+  function {:concurrent} GoodFn(b: Box<int>): int {
+    42
+  }
+
+  function {:concurrent} BadFn(b: Box<int>): int  // Error: reads clause might not be empty ({:concurrent} restriction)
+    reads b
+  {
+    b.x
+  }
+
+  function {:concurrent} WeirdButOkayFn(b: Box<int>): int 
+    reads if false then {b} else {}
+  {
+    42
+  }
+
+  method {:concurrent} GoodM(b: Box<int>) {
+  }
+
+  method {:concurrent} BadM(b: Box<int>)  // Error: reads clause might not be empty ({:concurrent} restriction)
+    reads b
+  {
+    var x := b.x;
+  }
+
+  method {:concurrent} WeirdButOkayM(b: Box<int>) 
+    reads if false then {b} else {}
+  {
+  }
+
+  method {:concurrent} AlsoBadM(b: Box<int>)  // Error: modifies clause might not be empty ({:concurrent} restriction)
+    modifies b
+  {
+    b.x := 42;
+  }
+
+  method {:concurrent} AlsoWeirdButOkayM(b: Box<int>) 
+    modifies if false then {b} else {}
+  {
+  }
+}
